src/Bedrock/Field/Synthesis/Examples/BLS12_G1_alt.v
@@ -1,3 +1,4 @@
+Require Import Crypto.Arithmetic.PrimeFieldTheorems.
 Require Import Crypto.Bedrock.Field.Synthesis.New.WordByWordMontgomery.
 Require Import Crypto.Bedrock.Field.Synthesis.Examples.bls12_prime.
 Require Import Crypto.Bedrock.Group.CurveAdd.CurveAddAlt.
@@ -12,42 +13,34 @@ Import Syntax BinInt String List.ListNotations.
 Local Open Scope string_scope. Local Open Scope Z_scope. Local Open Scope list_scope.
 Require Import Crypto.Bedrock.Field.FieldExtensions.QuadraticFieldExtensionsSpecs.
 Require Import Rupicola.Lib.Api.
-Require Import Crypto.Bedrock.Specs.AbstractField.
-Require Import Crypto.Bedrock.Specs.PrimeField.
+Require Import Crypto.Bedrock.Specs.Field.
 Require Import Crypto.Bedrock.Field.FieldExtensions.Theory.QuadraticExtensions.
-Require Import Crypto.Bedrock.Field.Interface.Compilation2.
+Require Import Crypto.Bedrock.Field.Interface.AbstracCompilation.
 Require Import Crypto.Arithmetic.UniformWeight.
 Require Import Crypto.Bedrock.Field.Translation.Parameters.Defaults64.
 Require Import Crypto.Bedrock.Field.Synthesis.Examples.BLS12_G1.
 
 Section bls12_Fp2.
 
-    Existing Instances Defaults64.default_parameters Defaults64.default_parameters_ok.
+  Existing Instances
+    Defaults64.default_parameters
+    Defaults64.default_parameters_ok.
 
-    Instance prime_field_parameters : PrimeField.PrimeFieldParameters.
-    Proof.
-        exact bls12_prime.field_parameters.
-    Defined.
-
-    Instance field_parameters : AbstractField.FieldParameters.
-    Proof.
-        exact (@PrimeField.prime_field_parameters prime_field_parameters).
-    Defined.
-
-    Instance field_representation : @AbstractField.FieldRepresentation field_parameters _ _ _ _.
-    Proof.
-        exact (WordByWordMontgomery.field_representation m).
-    Defined.
+  Existing Instances
+    bls12_prime_parameters
+    bls12_field_names
+    bls12_field_parameters
+    bls12_field_representation.
 
     Check @ladderstep_body. (*Give Proper Name!!!!!!!!*)
 
     Definition bls12_G1_add := ladderstep_body.
-    (*make AbstractField.field_representation from rep in WordByWordMontgomery.*)
+    (*make Field.field_representation from rep in WordByWordMontgomery.*)
 
-    Definition mpos : positive.
-    Proof.
-        destruct bls12_Fp2.prime_field_parameters. eapply M_pos.
-    Defined.
+    (* Definition mpos : positive. *)
+    (* Proof. *)
+    (*     destruct bls12_Fp2.prime_field_parameters. eapply M_pos. *)
+    (* Defined. *)
 
     (*hard-code curve-defining parameter b*)
     Definition b := 4.
@@ -56,7 +49,7 @@ Section bls12_Fp2.
     Definition n := felem_size_in_words.
     Definition three_b_list := Partition.partition uw n three_b.
     Definition word := BasicC64Semantics.word.
-    Definition three_b_mont := @WordByWordMontgomery.to_montgomerymod 64 n m (@m' prime_field_parameters 64) three_b_list.
+    Definition three_b_mont := @WordByWordMontgomery.to_montgomerymod 64 n M (@m' _ 64) three_b_list.
     Definition three_b_words := List.map (@word.of_Z 64 word) three_b_mont.
 
     Instance spec_of_bls12_add : spec_of (fst bls12_add).
@@ -77,12 +70,12 @@ Section bls12_Fp2.
     (* Instance spec_of_bls12_square : spec_of (fst bls12_square).
     Proof. exact spec_of_square. Defined. *)
 
-    Instance spec_of_G1_add : spec_of "ladderstep".
+    Instance spec_of_G1_add : spec_of "curve_add".
     Proof.
         exact (spec_of_ladderstep three_b_words).
     Defined.
 
-    Definition three_b_F : (@F field_parameters).
+    Definition three_b_F : (F M_pos).
     Proof.
         exact (ModularArithmetic.F.of_Z M_pos three_b).
     Defined.
@@ -92,10 +85,7 @@ Section bls12_Fp2.
         exact (spec_of_from_list).
     Defined.
 
-    Instance spec_of_bls12_felem_copy : spec_of ((@felem_copy bls12_prime.field_parameters)).
-    Proof.
-        exact (@spec_of_felem_copy _ _ _ _ _ _ field_parameters (field_representation )).
-    Defined.
+    Instance spec_of_bls12_felem_copy : spec_of felem_copy := spec_of_felem_copy.
 
     Instance spec_of_G1_add_alt : spec_of "G1_add_alt".
     Proof.
@@ -119,14 +109,14 @@ Section bls12_Fp2.
             stackalloc felem_size_in_bytes as allocy2;
             stackalloc felem_size_in_bytes as allocz1;
             stackalloc felem_size_in_bytes as allocz2;
-            coq:(cmd.call [] ((@felem_copy bls12_prime.field_parameters)) [expr.var ("allocx1"); expr.var ("x1")]);
-            coq:(cmd.call [] ((@felem_copy bls12_prime.field_parameters)) [expr.var ("allocx2"); expr.var ("x2")]);
-            coq:(cmd.call [] ((@felem_copy bls12_prime.field_parameters)) [expr.var ("allocy1"); expr.var ("y1")]);
-            coq:(cmd.call [] ((@felem_copy bls12_prime.field_parameters)) [expr.var ("allocy2"); expr.var ("y2")]);
-            coq:(cmd.call [] ((@felem_copy bls12_prime.field_parameters)) [expr.var ("allocz1"); expr.var ("z1")]);
-            coq:(cmd.call [] ((@felem_copy bls12_prime.field_parameters)) [expr.var ("allocz2"); expr.var ("z2")]);
+            coq:(cmd.call [] felem_copy [expr.var ("allocx1"); expr.var ("x1")]);
+            coq:(cmd.call [] felem_copy [expr.var ("allocx2"); expr.var ("x2")]);
+            coq:(cmd.call [] felem_copy [expr.var ("allocy1"); expr.var ("y1")]);
+            coq:(cmd.call [] felem_copy [expr.var ("allocy2"); expr.var ("y2")]);
+            coq:(cmd.call [] felem_copy [expr.var ("allocz1"); expr.var ("z1")]);
+            coq:(cmd.call [] felem_copy [expr.var ("allocz2"); expr.var ("z2")]);
             
-            coq:(cmd.call [] ("ladderstep") [expr.var ("allocx1"); expr.var ("allocx2"); expr.var ("allocy1"); expr.var("allocy2"); expr.var ("allocz1"); expr.var ("allocz2"); expr.var ("outx"); expr.var ("outy"); expr.var ("outz")])
+            coq:(cmd.call [] ("curve_add") [expr.var ("allocx1"); expr.var ("allocx2"); expr.var ("allocy1"); expr.var("allocy2"); expr.var ("allocz1"); expr.var ("allocz2"); expr.var ("outx"); expr.var ("outy"); expr.var ("outz")])
         ))).
 
         (*Proof alternate version*)
@@ -161,25 +151,22 @@ Section bls12_Fp2.
             repeat (erewrite map.get_put_diff; [| intros contra; discriminate]); eapply map.get_put_same|
         ]); repeat straightline.
 
-    Lemma alloc_to_FElem' : forall R m a l, Datatypes.length l = 48%nat -> (R * (array ptsto (word.of_Z 1) a l))%sep m -> exists f, (R * AbstractField.FElem a f)%sep m.
+    Lemma alloc_to_FElem' : forall R m a l, Datatypes.length l = 48%nat -> (R * (array ptsto (word.of_Z 1) a l))%sep m -> exists f, (R * Field.FElem a f)%sep m.
     Proof.
         intros. destruct H0, H0, H0, H1.
         do 3 eexists. split; eauto; split; eauto.
-        cbv [AbstractField.FElem].
+        cbv [Field.FElem].
         eapply Bignum.Bignum_of_bytes in H2.
             - simpl in H2. eapply H2.
             - auto.
     Qed.
 
+    Lemma bls12_G1_alt_ok : program_logic_goal_for_function! G1_add_alt.
 
-
-
-    Lemma bls12_G1_alt_ok : program_logic_goal_for_function! G1_add_alt. (*Why does this take 17 minutes??!?!?*)
-   
     pose proof ladderstep_correct.
     enter' G1_add_alt. clear H0 H1 H2 H3 H4. cbv [binop_spec spec_of_curve_add_alt] in *.
     intros.
-    do 9 (
+    do 7 (
         let bounds := (fresh "Hbounds") in
          destruct H0 as [bounds H0]
     ).    
@@ -278,273 +265,366 @@ Section bls12_Fp2.
         remember (AbstractField.FElem a3 x3) as P3.
         remember (AbstractField.FElem a4 x4) as P4.
 
-    
-        eassert ((_ * (P * P0 * P1 * P2 * P3 * P4))%sep a9) by ecancel_assumption.
-        remember ((P * P0 * P1 * P2 * P3 * P4))%sep as P5. clear H24 H25 H8 H26.
+    (*first alloc*)
+    (* esplit; compile_step. *)
+    (* esplit; compile_step. *)
+    (* esplit; compile_step. *)
+    (* esplit; compile_step. *)
+    (* esplit; compile_step. *)
+    repeat straightline.
+
+    straightline_call.
+    (* compile_step. *)
+    (* Admitted. *)
+
+    (* split; [apply Hmod|repeat straightline]. *)
+    (* split; [apply Hmod|repeat straightline]. *)
+    (* split; [apply Hmod|repeat straightline]. *)
+    (* split; [apply Hmod|repeat straightline]. *)
+    (* split; [apply Hmod|repeat straightline]. *)
+    (* split; [apply Hmod|repeat straightline]. *)
+    (* (* split; [apply Hmod| ]. repeat straightline. eapply alloc_to_FElem' in H2. *) *)
+    (* split; [apply Hmod| ]. repeat straightline. eapply alloc_to_FElem' in H15. *)
+    (* split; [apply Hmod| ]. repeat straightline. eapply alloc_to_FElem' in H13. *)
+    (* split; [apply Hmod| ]. repeat straightline. eapply alloc_to_FElem' in H32. *)
+    (* split; [apply Hmod| ]. repeat straightline. eapply alloc_to_FElem' in H47. *)
+    (* split; [apply Hmod| ]. repeat straightline. eapply alloc_to_FElem' in H64. *)
+
+    (* cbv [CurveAddAlt.my_field_representation] in *. *)
+    (* destruct H64. *)
+
+(*     straightline_call. *)
+    1: {
+        remember ((Field.FElem a x)) as P.
+        remember (Field.FElem a0 x0) as P0.
+        remember (Field.FElem a1 x1) as P1.
+        remember (Field.FElem a2 x2) as P2.
+        remember (Field.FElem a3 x3) as P3.
+        remember (Field.FElem a4 x4) as P4.
+
+
+        eassert ((_ * (P * P0 * P1 * P2 * P3 * P4))%sep mem) by ecancel_assumption.
+        remember ((P * P0 * P1 * P2 * P3 * P4))%sep as P5. clear H8.
         split; [| subst; ecancel_assumption].
         rename H21 into H8.
-        eapply sep_and_l_fwd in H8; destruct H8 as [? H8]; eapply sep_and_l_fwd in H8; destruct H8 as [H8 ?]; subst; ecancel_assumption.        
+        eapply sep_and_l_fwd in H8; destruct H8 as [? H8]; eapply sep_and_l_fwd in H8; destruct H8 as [H8 ?]; subst; ecancel_assumption.
       }
-    repeat straightline.
 
-    straightline_call.
-    1: {
-        remember ((AbstractField.FElem a X1)) as P.
-        remember (AbstractField.FElem a0 X2) as P0.
-        remember (AbstractField.FElem a1 Y1) as P1.
-        remember (AbstractField.FElem a2 Y2) as P2.
-        remember (AbstractField.FElem a3 x3) as P3.
-        remember (AbstractField.FElem a4 x4) as P4.
-
-    
-        eassert ((_ * (P * P0 * P1 * P2 * P3 * P4))%sep a10) by ecancel_assumption.
-        remember ((P * P0 * P1 * P2 * P3 * P4))%sep as P5. clear H24 H25 H8 H26 H27.
-        split; [| subst; ecancel_assumption].
-        rename H21 into H8.
-        eapply sep_and_l_fwd in H8; destruct H8 as [? H8]; eapply sep_and_l_fwd in H8; destruct H8 as [H8 ?]; subst; ecancel_assumption.        
-      }
-    repeat straightline.
-
-    straightline_call.
-    1: {
-        remember ((AbstractField.FElem a X1)) as P.
-        remember (AbstractField.FElem a0 X2) as P0.
-        remember (AbstractField.FElem a1 Y1) as P1.
-        remember (AbstractField.FElem a2 Y2) as P2.
-        remember (AbstractField.FElem a3 Z1) as P3.
-        remember (AbstractField.FElem a4 x4) as P4.
-
-    
-        eassert ((_ * (P * P0 * P1 * P2 * P3 * P4))%sep a11) by ecancel_assumption.
-        remember ((P * P0 * P1 * P2 * P3 * P4))%sep as P5. clear H24 H25 H8 H26 H27 H28.
-        split; [| subst; ecancel_assumption].
-        rename H21 into H8.
-        eapply sep_and_l_fwd in H8; destruct H8 as [? H8]; eapply sep_and_l_fwd in H8; destruct H8 as [H8 ?]; subst; ecancel_assumption.        
-      }
-    repeat straightline.
-
-    straightline_call.
-    1: {
-        remember ((AbstractField.FElem a X1)) as P.
-        remember (AbstractField.FElem a0 X2) as P0.
-        remember (AbstractField.FElem a1 Y1) as P1.
-        remember (AbstractField.FElem a2 Y2) as P2.
-        remember (AbstractField.FElem a3 Z1) as P3.
-        remember (AbstractField.FElem a4 Z2) as P4.
-
-    
-        eassert ((_ * (P * P0 * P1 * P2 * P3 * P4))%sep a12) by ecancel_assumption.
-        remember ((P * P0 * P1 * P2 * P3 * P4))%sep as P5. clear H24 H25 H8 H26 H27 H28 H29.
-        rename H21 into H8.
-        eapply sep_and_l_fwd in H8; destruct H8 as [? H8]; eapply sep_and_l_fwd in H8; destruct H8 as [H8 ?].
-        subst.
+(*     repeat straightline. *)
 
 
-        Lemma FElem_to_FElem' : forall a m l, bounded_by tight_bounds l -> AbstractField.FElem a l m -> CompilationAbstract.FElem (Some tight_bounds) a (feval l) m.
-        Proof.
-            intros. cbv [CompilationAbstract.FElem]. cbv [Lift1Prop.ex1]. eexists. sepsimpl.
-                3: ecancel_assumption.
-                all: auto.
-        Qed.
-
-        Lemma FElem_to_FElem'_R : forall a m l R, bounded_by tight_bounds l -> (AbstractField.FElem a l * R)%sep m -> (R * CompilationAbstract.FElem (Some tight_bounds) a (feval l))%sep m.
-        Proof.
-            intros. destruct H0, H0, H0, H1. eapply map.split_comm in H0.
-            eexists; eexists; split; eauto. split; eauto.
-            eapply FElem_to_FElem'; eauto.
-        Qed.
-
-        Lemma FElem_to_FElem'_R' : forall a m l R1 R2, bounded_by tight_bounds l -> (R1 * AbstractField.FElem a l * R2)%sep m -> (R1 * R2 * CompilationAbstract.FElem (Some tight_bounds) a (feval l))%sep m.
-        Proof.
-            intros.
-            eapply sep_comm in H0. eapply sep_assoc in H0.
-            destruct H0, H0, H0, H1.
-            eexists; eexists; split; eauto. split; [eapply sep_comm| ]; eauto.
-            eapply FElem_to_FElem'; eauto.
-        Qed.
-
-        eassert ((Rout * _)%sep a12) by ecancel_assumption. clear H21.
-        destruct H24, H21, H21, H24.
-        eexists; eexists; split.
-        1: eapply map.split_comm; eapply H21.
-        split; [| eapply H24].
-
-        eapply FElem_to_FElem'_R; cycle -1.
-        1: eapply (sep_assoc (AbstractField.FElem _ _)); eapply FElem_to_FElem'_R; cycle -1.
-        1:  eapply (sep_assoc (AbstractField.FElem _ _));
-            eapply (sep_assoc (AbstractField.FElem _ _ * AbstractField.FElem _ _)%sep);
-            eapply FElem_to_FElem'_R; cycle -1.
-
-        1:  eapply (sep_assoc (AbstractField.FElem _ _));
-            eapply (sep_assoc (AbstractField.FElem _ _ * (AbstractField.FElem _ _ * AbstractField.FElem _ _))%sep);
-            eapply FElem_to_FElem'_R; cycle -1.
-
-        1:  eapply (sep_assoc (AbstractField.FElem _ _)).
-            eapply (sep_assoc (AbstractField.FElem _ _ * (AbstractField.FElem _ _ * (AbstractField.FElem _ _ * AbstractField.FElem _ _)))%sep);
-            eapply FElem_to_FElem'_R; cycle -1.
-
-        1:  eapply (sep_assoc (AbstractField.FElem _ _)).
-            eapply (sep_assoc (AbstractField.FElem _ _ * (AbstractField.FElem _ _ * (AbstractField.FElem _ _ * (AbstractField.FElem _ _ * AbstractField.FElem _ _))))%sep);
-            eapply FElem_to_FElem'_R; cycle -1.
-
-        1:  eapply (sep_assoc (AbstractField.FElem _ _)).
-            eapply (sep_assoc (AbstractField.FElem _ _ * (AbstractField.FElem _ _ * (AbstractField.FElem _ _ * (AbstractField.FElem _ _ * (AbstractField.FElem _ _ * AbstractField.FElem _ _)))))%sep);
-            eapply FElem_to_FElem'_R; cycle -1.
-
-        1:  eapply (sep_assoc (AbstractField.FElem _ _)).
-            eapply (sep_assoc (AbstractField.FElem _ _ * (AbstractField.FElem _ _ * (AbstractField.FElem _ _ * (AbstractField.FElem _ _ * (AbstractField.FElem _ _ * (AbstractField.FElem _ _ * AbstractField.FElem _ _))))))%sep);
-            eapply FElem_to_FElem'_R; cycle -1.
-
-        1:  eapply (sep_assoc (AbstractField.FElem _ _)).
-        1:  eapply FElem_to_FElem'_R.
-
-        2: ecancel_assumption.
-
-        all: eassumption.
-    }
-
-    repeat straightline.
-    clear H29 H28 H27 H26 H25 H24 H8.
-    {
-        cbv [my_field_representation bls12_Fp2.word] in *.
-        eassert (Htemp : (CompilationAbstract.FElem (Some tight_bounds) a4 (feval Z2) * _)%sep a13) by ecancel_assumption. clear H31. rename Htemp into H31.
-        do 4 destruct H31 as [? H31].
-    }
-    eexists. eexists. split; [eauto| split].
-    
-    2: {
-
-    }
-    
-    [eauto| ]. repeat straightline.
-    split; [eauto| ].
+(*     straightline_call. *)
+(*     1: { *)
+(*         remember ((Field.FElem a X1)) as P. *)
+(*         remember (Field.FElem a0 x0) as P0. *)
+(*         remember (Field.FElem a1 x1) as P1. *)
+(*         remember (Field.FElem a2 x2) as P2. *)
+(*         remember (Field.FElem a3 x3) as P3. *)
+(*         remember (Field.FElem a4 x4) as P4. *)
 
 
+(*         eassert ((_ * (P * P0 * P1 * P2 * P3 * P4))%sep a6) by ecancel_assumption. *)
+(*         remember ((P * P0 * P1 * P2 * P3 * P4))%sep as P5. clear H24. clear H8. *)
+(*         split; [| subst; ecancel_assumption]. *)
+(*         rename H21 into H8. *)
+(*         eapply sep_and_l_fwd in H8; destruct H8 as [? H8]; eapply sep_and_l_fwd in H8; destruct H8 as [H8 ?]; subst; ecancel_assumption.         *)
+(*       } *)
+(*     repeat straightline. *)
+
+(*     straightline_call. *)
+(*     1: { *)
+(*         remember ((Field.FElem a X1)) as P. *)
+(*         remember (Field.FElem a0 X2) as P0. *)
+(*         remember (Field.FElem a1 x1) as P1. *)
+(*         remember (Field.FElem a2 x2) as P2. *)
+(*         remember (Field.FElem a3 x3) as P3. *)
+(*         remember (Field.FElem a4 x4) as P4. *)
 
 
-        cbv [CompilationAbstract.FElem]. sepsimpl.
-        Search (Lift1Prop.ex1).
-        
-        ecancel_assumption.
-        subst; ecancel_assumption.        
-      }
-    repeat straightline.
-    
+(*         eassert ((_ * (P * P0 * P1 * P2 * P3 * P4))%sep a8) by ecancel_assumption. *)
+(*         remember ((P * P0 * P1 * P2 * P3 * P4))%sep as P5. clear H24 H25 H8. *)
+(*         split; [| subst; ecancel_assumption]. *)
+(*         rename H21 into H8. *)
+(*         eapply sep_and_l_fwd in H8; destruct H8 as [? H8]; eapply sep_and_l_fwd in H8; destruct H8 as [H8 ?]; subst; ecancel_assumption.         *)
+(*       } *)
+(*     repeat straightline. *)
+
+(*     straightline_call. *)
+(*     1: { *)
+(*         remember ((Field.FElem a X1)) as P. *)
+(*         remember (Field.FElem a0 X2) as P0. *)
+(*         remember (Field.FElem a1 Y1) as P1. *)
+(*         remember (Field.FElem a2 x2) as P2. *)
+(*         remember (Field.FElem a3 x3) as P3. *)
+(*         remember (Field.FElem a4 x4) as P4. *)
 
 
-    eapply Proper_call.
-    {
-        cbv [pointwise_relation]. repeat straightline. cbv [Basics.impl]. repeat straightline.
-        eexists. split.
-        1: solve_locals7 l5 l4 l3 l2 l1 l0 l.
-        {
-            subst l5 l4 l3 l2 l1 l0 l. simpl.
-        }
-        subst l5. subst l4. subst l3. subst l2. subst l1.
-    }
+(*         eassert ((_ * (P * P0 * P1 * P2 * P3 * P4))%sep a9) by ecancel_assumption. *)
+(*         remember ((P * P0 * P1 * P2 * P3 * P4))%sep as P5. clear H24 H25 H8 H26. *)
+(*         split; [| subst; ecancel_assumption]. *)
+(*         rename H21 into H8. *)
+(*         eapply sep_and_l_fwd in H8; destruct H8 as [? H8]; eapply sep_and_l_fwd in H8; destruct H8 as [H8 ?]; subst; ecancel_assumption.         *)
+(*       } *)
+(*     repeat straightline. *)
+
+(*     straightline_call. *)
+(*     1: { *)
+(*         remember ((Field.FElem a X1)) as P. *)
+(*         remember (Field.FElem a0 X2) as P0. *)
+(*         remember (Field.FElem a1 Y1) as P1. *)
+(*         remember (Field.FElem a2 Y2) as P2. *)
+(*         remember (Field.FElem a3 x3) as P3. *)
+(*         remember (Field.FElem a4 x4) as P4. *)
+
+
+(*         eassert ((_ * (P * P0 * P1 * P2 * P3 * P4))%sep a10) by ecancel_assumption. *)
+(*         remember ((P * P0 * P1 * P2 * P3 * P4))%sep as P5. clear H24 H25 H8 H26 H27. *)
+(*         split; [| subst; ecancel_assumption]. *)
+(*         rename H21 into H8. *)
+(*         eapply sep_and_l_fwd in H8; destruct H8 as [? H8]; eapply sep_and_l_fwd in H8; destruct H8 as [H8 ?]; subst; ecancel_assumption.         *)
+(*       } *)
+(*     repeat straightline. *)
+
+(*     straightline_call. *)
+(*     1: { *)
+(*         remember ((Field.FElem a X1)) as P. *)
+(*         remember (Field.FElem a0 X2) as P0. *)
+(*         remember (Field.FElem a1 Y1) as P1. *)
+(*         remember (Field.FElem a2 Y2) as P2. *)
+(*         remember (Field.FElem a3 Z1) as P3. *)
+(*         remember (Field.FElem a4 x4) as P4. *)
+
+
+(*         eassert ((_ * (P * P0 * P1 * P2 * P3 * P4))%sep a11) by ecancel_assumption. *)
+(*         remember ((P * P0 * P1 * P2 * P3 * P4))%sep as P5. clear H24 H25 H8 H26 H27 H28. *)
+(*         split; [| subst; ecancel_assumption]. *)
+(*         rename H21 into H8. *)
+(*         eapply sep_and_l_fwd in H8; destruct H8 as [? H8]; eapply sep_and_l_fwd in H8; destruct H8 as [H8 ?]; subst; ecancel_assumption.         *)
+(*       } *)
+(*     repeat straightline. *)
+
+(*     straightline_call. *)
+(*     1: { *)
+(*         remember ((Field.FElem a X1)) as P. *)
+(*         remember (Field.FElem a0 X2) as P0. *)
+(*         remember (Field.FElem a1 Y1) as P1. *)
+(*         remember (Field.FElem a2 Y2) as P2. *)
+(*         remember (Field.FElem a3 Z1) as P3. *)
+(*         remember (Field.FElem a4 Z2) as P4. *)
+
+
+(*         eassert ((_ * (P * P0 * P1 * P2 * P3 * P4))%sep a12) by ecancel_assumption. *)
+(*         remember ((P * P0 * P1 * P2 * P3 * P4))%sep as P5. clear H24 H25 H8 H26 H27 H28 H29. *)
+(*         rename H21 into H8. *)
+(*         eapply sep_and_l_fwd in H8; destruct H8 as [? H8]; eapply sep_and_l_fwd in H8; destruct H8 as [H8 ?]. *)
+(*         subst. *)
+
+
+(*         Lemma FElem_to_FElem' : forall a m l, bounded_by tight_bounds l -> Field.FElem a l m -> CompilationAbstract.FElem (Some tight_bounds) a (feval l) m. *)
+(*         Proof. *)
+(*             intros. cbv [CompilationAbstract.FElem]. cbv [Lift1Prop.ex1]. eexists. sepsimpl. *)
+(*                 3: ecancel_assumption. *)
+(*                 all: auto. *)
+(*         Qed. *)
+
+(*         Lemma FElem_to_FElem'_R : forall a m l R, bounded_by tight_bounds l -> (Field.FElem a l * R)%sep m -> (R * CompilationAbstract.FElem (Some tight_bounds) a (feval l))%sep m. *)
+(*         Proof. *)
+(*             intros. destruct H0, H0, H0, H1. eapply map.split_comm in H0. *)
+(*             eexists; eexists; split; eauto. split; eauto. *)
+(*             eapply FElem_to_FElem'; eauto. *)
+(*         Qed. *)
+
+(*         Lemma FElem_to_FElem'_R' : forall a m l R1 R2, bounded_by tight_bounds l -> (R1 * Field.FElem a l * R2)%sep m -> (R1 * R2 * CompilationAbstract.FElem (Some tight_bounds) a (feval l))%sep m. *)
+(*         Proof. *)
+(*             intros. *)
+(*             eapply sep_comm in H0. eapply sep_assoc in H0. *)
+(*             destruct H0, H0, H0, H1. *)
+(*             eexists; eexists; split; eauto. split; [eapply sep_comm| ]; eauto. *)
+(*             eapply FElem_to_FElem'; eauto. *)
+(*         Qed. *)
+
+(*         eassert ((Rout * _)%sep a12) by ecancel_assumption. clear H21. *)
+(*         destruct H24, H21, H21, H24. *)
+(*         eexists; eexists; split. *)
+(*         1: eapply map.split_comm; eapply H21. *)
+(*         split; [| eapply H24]. *)
+
+(*         eapply FElem_to_FElem'_R; cycle -1. *)
+(*         1: eapply (sep_assoc (Field.FElem _ _)); eapply FElem_to_FElem'_R; cycle -1. *)
+(*         1:  eapply (sep_assoc (Field.FElem _ _)); *)
+(*             eapply (sep_assoc (Field.FElem _ _ * Field.FElem _ _)%sep); *)
+(*             eapply FElem_to_FElem'_R; cycle -1. *)
+
+(*         1:  eapply (sep_assoc (Field.FElem _ _)); *)
+(*             eapply (sep_assoc (Field.FElem _ _ * (Field.FElem _ _ * Field.FElem _ _))%sep); *)
+(*             eapply FElem_to_FElem'_R; cycle -1. *)
+
+(*         1:  eapply (sep_assoc (Field.FElem _ _)). *)
+(*             eapply (sep_assoc (Field.FElem _ _ * (Field.FElem _ _ * (Field.FElem _ _ * Field.FElem _ _)))%sep); *)
+(*             eapply FElem_to_FElem'_R; cycle -1. *)
+
+(*         1:  eapply (sep_assoc (Field.FElem _ _)). *)
+(*             eapply (sep_assoc (Field.FElem _ _ * (Field.FElem _ _ * (Field.FElem _ _ * (Field.FElem _ _ * Field.FElem _ _))))%sep); *)
+(*             eapply FElem_to_FElem'_R; cycle -1. *)
+
+(*         1:  eapply (sep_assoc (Field.FElem _ _)). *)
+(*             eapply (sep_assoc (Field.FElem _ _ * (Field.FElem _ _ * (Field.FElem _ _ * (Field.FElem _ _ * (Field.FElem _ _ * Field.FElem _ _)))))%sep); *)
+(*             eapply FElem_to_FElem'_R; cycle -1. *)
+
+(*         1:  eapply (sep_assoc (Field.FElem _ _)). *)
+(*             eapply (sep_assoc (Field.FElem _ _ * (Field.FElem _ _ * (Field.FElem _ _ * (Field.FElem _ _ * (Field.FElem _ _ * (Field.FElem _ _ * Field.FElem _ _))))))%sep); *)
+(*             eapply FElem_to_FElem'_R; cycle -1. *)
+
+(*         1:  eapply (sep_assoc (Field.FElem _ _)). *)
+(*         1:  eapply FElem_to_FElem'_R. *)
+
+(*         2: ecancel_assumption. *)
+
+(*         all: eassumption. *)
+(*     } *)
+
+(*     repeat straightline. *)
+(*     clear H29 H28 H27 H26 H25 H24 H8. *)
+(*     { *)
+(*         cbv [my_field_representation bls12_Fp2.word] in *. *)
+(*         eassert (Htemp : (CompilationAbstract.FElem (Some tight_bounds) a4 (feval Z2) * _)%sep a13) by ecancel_assumption. clear H31. rename Htemp into H31. *)
+(*         do 4 destruct H31 as [? H31]. *)
+(*     } *)
+(*     eexists. eexists. split; [eauto| split]. *)
+
+(*     2: { *)
+
+(*     } *)
+
+(*     [eauto| ]. repeat straightline. *)
+(*     split; [eauto| ]. *)
+
+
+
+
+(*         cbv [CompilationAbstract.FElem]. sepsimpl. *)
+(*         Search (Lift1Prop.ex1). *)
+
+(*         ecancel_assumption. *)
+(*         subst; ecancel_assumption.         *)
+(*       } *)
+(*     repeat straightline. *)
+
+
+
+(*     eapply Proper_call. *)
+(*     { *)
+(*         cbv [pointwise_relation]. repeat straightline. cbv [Basics.impl]. repeat straightline. *)
+(*         eexists. split. *)
+(*         1: solve_locals7 l5 l4 l3 l2 l1 l0 l. *)
+(*         { *)
+(*             subst l5 l4 l3 l2 l1 l0 l. simpl. *)
+(*         } *)
+(*         subst l5. subst l4. subst l3. subst l2. subst l1. *)
+(*     } *)
 
 
 
 
 
-    eexists.
-    
-    {
+(*     eexists. *)
 
-    }
-    
-    cbv [spec_of_G1_add].
-    cbv [G1_add_alt].
-    cbv [program_logic_goal_for]. intros.
-    cbv [spec_of_G1_add_alt].
-    cbv [spec_of_curve_add_alt].
-    repeat straightline.
-    eapply Proper_call.
-    {
-        cbv [pointwise_relation]. repeat straightline. cbv [Basics.impl]. intros. split.
-        simpl.
-    }
-    straightline_call.
-    eapply H.
-        1: simpl; auto.
-        3: auto.
-        3: cbv [spec_of_bls12_add] in H4; apply H4.
-        3: cbv [spec_of_bls12_sub] in H13; apply H13.
-        2: {
-            cbv [__rupicola_program_marker]. auto.
-        }
-        2: {
-            cbv [CurveAdd.spec_of_from_list]. cbv [spec_of_from_list] in H0.
-            assert (three_b_F = feval three_b_words).
-            {
-                simpl. cbv [Representation.eval_words eval_trans three_b_F].
-                Require Import Crypto.Bedrock.Field.Synthesis.Examples.bls12_from_list_F.
-                pose proof (three_b_mont_mod).
-                assert (three_b_words = bls12_Fp2.three_b_words).
-                {
-                    cbv [bls12_Fp2.three_b_words three_b_words]. eapply f_equal.
-                    cbv [bls12_Fp2.three_b_mont three_b_mont bls12_Fp2.three_b_list].
-                    cbv. reflexivity.
-                }
-                rewrite <- H35.
-                apply f_equal.
-                cbv [word] in H34.
-                assert (@M bls12_prime.field_parameters = m).
-                {
-                    simpl. cbv [M]. cbv [m]. cbv [M_pos]. simpl. reflexivity.
-                }
-                rewrite H36 in H34.
-                rewrite H34.
-                cbv [three_b_list]. rewrite eval_partition; [| eapply uwprops].
-                2 : {
-                    clear H H1 H2 H4 H6 H7 H9 H10 H11 H12 H13 H14 H15 H16 H17 H18 H19 H20 H21 H22 H23 H24 H25 H26 H27 H28 H29 H30 H31 H32 H33.
-                    clear H34 H35 H36. lia.
-                }
-                clear H H1 H2 H4 H6 H7 H9 H10 H11 H12 H13 H14 H15 H16 H17 H18 H19 H20 H21 H22 H23 H24 H25 H26 H27 H28 H29 H30 H31 H32 H33.
-                cbv [three_b bls12_Fp2.three_b]. erewrite Zmod_small; try lia.
-                cbv [n felem_size_in_words]. simpl. cbv [WordByWordMontgomery.n]. simpl.
-                cbv [uw uweight ModOps.weight]. simpl. lia.
-            }
-            rewrite H34 in H0.
-            eapply H0.
-        }
-        clear H H1 H2 H4 H6 H7 H9 H10 H11 H12 H13 H14 H15 H16 H17 H18 H19 H20 H21 H22 H23 H24 H25 H26 H27 H28 H29 H30 H31 H32 H33.
-        cbv [CompilationAbstract.maybe_bounded bounded_by loose_bounds bls12_Fp2.three_b_words].
-        eassert (my_field_representation = _).
-        {
-            cbv [my_field_representation]. eauto. 
-        }
-        rewrite H.
-        eassert (bls12_Fp2.field_representation = _).
-        {
-            cbv [bls12_Fp2.field_representation]. auto.
-        }
-        cbv [bls12_Fp2.field_representation]. remember (List.map word.of_Z bls12_Fp2.three_b_mont) as eyy.
-        simpl. subst eyy.
+(*     { *)
+
+(*     } *)
+
+(*     cbv [spec_of_G1_add]. *)
+(*     cbv [G1_add_alt]. *)
+(*     cbv [program_logic_goal_for]. intros. *)
+(*     cbv [spec_of_G1_add_alt]. *)
+(*     cbv [spec_of_curve_add_alt]. *)
+(*     repeat straightline. *)
+(*     eapply Proper_call. *)
+(*     { *)
+(*         cbv [pointwise_relation]. repeat straightline. cbv [Basics.impl]. intros. split. *)
+(*         simpl. *)
+(*     } *)
+(*     straightline_call. *)
+(*     eapply H. *)
+(*         1: simpl; auto. *)
+(*         3: auto. *)
+(*         3: cbv [spec_of_bls12_add] in H4; apply H4. *)
+(*         3: cbv [spec_of_bls12_sub] in H13; apply H13. *)
+(*         2: { *)
+(*             cbv [__rupicola_program_marker]. auto. *)
+(*         } *)
+(*         2: { *)
+(*             cbv [CurveAdd.spec_of_from_list]. cbv [spec_of_from_list] in H0. *)
+(*             assert (three_b_F = feval three_b_words). *)
+(*             { *)
+(*                 simpl. cbv [Representation.eval_words eval_trans three_b_F]. *)
+(*                 Require Import Crypto.Bedrock.Field.Synthesis.Examples.bls12_from_list_F. *)
+(*                 pose proof (three_b_mont_mod). *)
+(*                 assert (three_b_words = bls12_Fp2.three_b_words). *)
+(*                 { *)
+(*                     cbv [bls12_Fp2.three_b_words three_b_words]. eapply f_equal. *)
+(*                     cbv [bls12_Fp2.three_b_mont three_b_mont bls12_Fp2.three_b_list]. *)
+(*                     cbv. reflexivity. *)
+(*                 } *)
+(*                 rewrite <- H35. *)
+(*                 apply f_equal. *)
+(*                 cbv [word] in H34. *)
+(*                 assert (@M bls12_prime.field_parameters = m). *)
+(*                 { *)
+(*                     simpl. cbv [M]. cbv [m]. cbv [M_pos]. simpl. reflexivity. *)
+(*                 } *)
+(*                 rewrite H36 in H34. *)
+(*                 rewrite H34. *)
+(*                 cbv [three_b_list]. rewrite eval_partition; [| eapply uwprops]. *)
+(*                 2 : { *)
+(*                     clear H H1 H2 H4 H6 H7 H9 H10 H11 H12 H13 H14 H15 H16 H17 H18 H19 H20 H21 H22 H23 H24 H25 H26 H27 H28 H29 H30 H31 H32 H33. *)
+(*                     clear H34 H35 H36. lia. *)
+(*                 } *)
+(*                 clear H H1 H2 H4 H6 H7 H9 H10 H11 H12 H13 H14 H15 H16 H17 H18 H19 H20 H21 H22 H23 H24 H25 H26 H27 H28 H29 H30 H31 H32 H33. *)
+(*                 cbv [three_b bls12_Fp2.three_b]. erewrite Zmod_small; try lia. *)
+(*                 cbv [n felem_size_in_words]. simpl. cbv [WordByWordMontgomery.n]. simpl. *)
+(*                 cbv [uw uweight ModOps.weight]. simpl. lia. *)
+(*             } *)
+(*             rewrite H34 in H0. *)
+(*             eapply H0. *)
+(*         } *)
+(*         clear H H1 H2 H4 H6 H7 H9 H10 H11 H12 H13 H14 H15 H16 H17 H18 H19 H20 H21 H22 H23 H24 H25 H26 H27 H28 H29 H30 H31 H32 H33. *)
+(*         cbv [CompilationAbstract.maybe_bounded bounded_by loose_bounds bls12_Fp2.three_b_words]. *)
+(*         eassert (my_field_representation = _). *)
+(*         { *)
+(*             cbv [my_field_representation]. eauto.  *)
+(*         } *)
+(*         rewrite H. *)
+(*         eassert (bls12_Fp2.field_representation = _). *)
+(*         { *)
+(*             cbv [bls12_Fp2.field_representation]. auto. *)
+(*         } *)
+(*         cbv [bls12_Fp2.field_representation]. remember (List.map word.of_Z bls12_Fp2.three_b_mont) as eyy. *)
+(*         simpl. subst eyy. *)
 
 
-        assert (three_b_mont = bls12_Fp2.three_b_mont).
-        {
-            pose proof (three_b_mont_eq). rewrite H2.
-            cbv [bls12_Fp2.three_b_mont bls12_Fp2.three_b_list bls12_Fp2.three_b].
-            cbv [three_b_list three_b].
-            assert (n = bls12_Fp2.n).
-            {
-                cbv [bls12_Fp2.n]. cbv [n]. reflexivity.
-            }
-            rewrite <- H4.
-            assert (bls12_Fp2.uw = uw).
-            {
-                cbv [bls12_Fp2.uw]. cbv [uw]. reflexivity.
-            }
-            rewrite H6. reflexivity.
-        }
-        rewrite <- H2.
-        rewrite unsigned_of_Z_valid.
+(*         assert (three_b_mont = bls12_Fp2.three_b_mont). *)
+(*         { *)
+(*             pose proof (three_b_mont_eq). rewrite H2. *)
+(*             cbv [bls12_Fp2.three_b_mont bls12_Fp2.three_b_list bls12_Fp2.three_b]. *)
+(*             cbv [three_b_list three_b]. *)
+(*             assert (n = bls12_Fp2.n). *)
+(*             { *)
+(*                 cbv [bls12_Fp2.n]. cbv [n]. reflexivity. *)
+(*             } *)
+(*             rewrite <- H4. *)
+(*             assert (bls12_Fp2.uw = uw). *)
+(*             { *)
+(*                 cbv [bls12_Fp2.uw]. cbv [uw]. reflexivity. *)
+(*             } *)
+(*             rewrite H6. reflexivity. *)
+(*         } *)
+(*         rewrite <- H2. *)
+(*         rewrite unsigned_of_Z_valid. *)
 
-        2: cbv [n felem_size_in_words]; simpl.
-        all: eapply three_b_mont_valid.
-Qed. *)
+(*         2: cbv [n felem_size_in_words]; simpl. *)
+(*         all: eapply three_b_mont_valid. *)
+(* Qed. *)
 
 End bls12_Fp2.
     (* From bedrock2 Require Import ToCString Bytedump.
